Test/Mono.lean
@@ -1,5 +1,29 @@
 import Nunchaku
 
+namespace Bar
+
+inductive Tree (α : Type) where
+| empty
+| node (xs : List (Tree α)) (n : α)
+
+def Tree.map (t : Tree α) (f : α → β) : Tree β :=
+  match t with
+  | .empty => .empty
+  | .node xs n => .node (xs.map (Tree.map · f)) (f n)
+
+/--
+info: The prover found a counter example
+---
+error: unsolved goals
+a b : Tree Nat
+⊢ a.map Nat.succ = a
+-/
+#guard_msgs in
+example (a b : Tree Nat) : a.map Nat.succ = a := by
+  nunchaku
+
+end Bar
+
 namespace Foo
 
 inductive MList (α : Type) where
@@ -127,15 +151,17 @@ example (xs : List Nat) (h : xs ≠ []) : sumalt' xs ≠ .zero := by
 
 def foo (xs : List α) : List α := id xs
 
-/--
-info: The prover is convinced that the theorem is true.
----
-error: unsolved goals
-α : Type u_1
-xs : List α
-⊢ foo xs = id xs
--/
-#guard_msgs in
+--/--
+--info: The prover is convinced that the theorem is true.
+-----
+--error: unsolved goals
+--α : Type u_1
+--xs : List α
+--⊢ foo xs = id xs
+---/
+--#guard_msgs in
+set_option Elab.async false
+set_option trace.nunchaku true in
 example (xs : List α) : foo xs = id xs := by
   nunchaku
 
@@ -153,7 +179,6 @@ h : xs = []
 example (xs : List α) (h : xs = []) : xs.all f = false := by
   nunchaku
 
-/-
 inductive MyAll {α : Type} (p : α → Prop) : List α → Prop where
   | nil : MyAll p []
   | cons (x : α) (xs : List α) (h1 : p x) (h2 : MyAll p xs) : MyAll p (x :: xs)
@@ -162,7 +187,6 @@ inductive MyAll {α : Type} (p : α → Prop) : List α → Prop where
 set_option trace.nunchaku true in
 example (xs : List α) (h : xs = []) : MyAll (fun _ => False) xs := by
   nunchaku
-  -/
 
 /-
 TODO: times out
